src/QueryStructure/Implementation/Constraints/ConstraintChecksRefinements.v
@@ -10,6 +10,7 @@ Require Import Coq.Lists.List Coq.Arith.Compare_dec Coq.Bool.Bool Coq.Strings.St
         Fiat.Common.List.ListFacts
         Fiat.Common.LogicFacts
         Fiat.Common.DecideableEnsembles
+        Fiat.Computation.Refinements.Iterate_Decide_Comp
         Fiat.QueryStructure.Specification.Constraints.tupleAgree
         Fiat.QueryStructure.Specification.Operations.Mutate.
 
@@ -23,72 +24,61 @@ Section ConstraintCheckRefinements.
        SatisfiesAttributeConstraints
        SatisfiesTupleConstraints.
 
-Fixpoint Tuple_Agree_eq'
-         {h : Heading}
-         {attrlist : list (Attributes h)}
-         (attr_eq_dec : ilist (fun attr => Query_eq (Domain h attr)) attrlist)
-         (tup tup' : @Tuple h)
-: bool :=
-  match attr_eq_dec with
-      | inil => true
-      | icons a attrlist' a_eq_dec attr_eq_dec' =>
-        if @A_eq_dec _ a_eq_dec (GetAttribute tup a) (GetAttribute tup' a)
-        then Tuple_Agree_eq' attr_eq_dec' tup tup'
-        else false
-  end.
+  Fixpoint Tuple_Agree_eq'
+           {h : Heading}
+           {attrlist : list (Attributes h)}
+           (attr_eq_dec : ilist (fun attr => Query_eq (Domain h attr)) attrlist)
+           (tup tup' : @Tuple h)
+    : bool :=
+    match attr_eq_dec with
+    | inil => true
+    | icons a attrlist' a_eq_dec attr_eq_dec' =>
+      if @A_eq_dec _ a_eq_dec (GetAttribute tup a) (GetAttribute tup' a)
+      then Tuple_Agree_eq' attr_eq_dec' tup tup'
+      else false
+    end.
 
-Program Fixpoint ilist_map {A C : Type} {B : C -> Type}
-           (As : list A)
-           (f : A -> C)
-           (il : ilist B (map f As))
-: ilist (fun a => B (f a)) As :=
-  match As as As' return ilist B (map f As') -> ilist (fun a => B (f a)) As' with
-      | nil => fun _ => inil _
-      | a :: As' => fun il => icons _ (ilist_hd il)
-                                    (ilist_map As' f (ilist_tl il))
-  end il.
+  Class List_Query_eq (As : list Type) :=
+    { As_Query_eq : ilist Query_eq As}.
 
-Class List_Query_eq (As : list Type) :=
-  { As_Query_eq : ilist Query_eq As}.
+  Program Definition Tuple_Agree_eq {h} (attrlist : list (Attributes h))
+          (attr_eq_dec : List_Query_eq (map (Domain h) attrlist)) tup tup' :=
+    Tuple_Agree_eq' (ilist_map _ _ (@As_Query_eq _ attr_eq_dec)) tup tup'.
 
-Program Definition Tuple_Agree_eq {h} (attrlist : list (Attributes h))
-        (attr_eq_dec : List_Query_eq (map (Domain h) attrlist)) tup tup' :=
-  Tuple_Agree_eq' (ilist_map _ _ (@As_Query_eq _ attr_eq_dec)) tup tup'.
+  Lemma Tuple_Agree_eq_dec h attrlist attr_eq_dec (tup tup' : @Tuple h) :
+    tupleAgree tup tup' attrlist <->
+    Tuple_Agree_eq attrlist attr_eq_dec tup tup' = true.
+  Proof.
+    destruct attr_eq_dec.
+    induction attrlist; unfold tupleAgree in *; simpl in *; simpl;
+    intuition;
+    unfold Tuple_Agree_eq in *; simpl in *; find_if_inside; simpl; subst; eauto;
+    try (eapply IHattrlist; eauto; fail);
+    discriminate.
+  Qed.
 
-Lemma Tuple_Agree_eq_dec h attrlist attr_eq_dec (tup tup' : @Tuple h) :
-  tupleAgree tup tup' attrlist <->
-  Tuple_Agree_eq attrlist attr_eq_dec tup tup' = true.
-Proof.
-  destruct attr_eq_dec.
-  induction attrlist; unfold tupleAgree in *; simpl in *; simpl;
-  intuition;
-  unfold Tuple_Agree_eq in *; simpl in *; find_if_inside; simpl; subst; eauto;
-  try (eapply IHattrlist; eauto; fail);
-  discriminate.
-Qed.
+  Lemma Tuple_Agree_eq_dec' h attrlist attr_eq_dec (tup tup' : @Tuple h) :
+    ~ tupleAgree tup tup' attrlist <->
+    Tuple_Agree_eq attrlist attr_eq_dec tup tup' = false.
+  Proof.
+    destruct attr_eq_dec.
+    induction attrlist; unfold tupleAgree in *; simpl in *; simpl;
+    intuition;
+    unfold Tuple_Agree_eq in *; simpl in *; intuition;
+    find_if_inside; simpl; subst; eauto.
+    try (eapply IHattrlist; intros; eapply H).
+    intros; intuition; subst; auto.
+    eapply IHattrlist; intros; eauto.
+  Qed.
 
-Lemma Tuple_Agree_eq_dec' h attrlist attr_eq_dec (tup tup' : @Tuple h) :
-  ~ tupleAgree tup tup' attrlist <->
-  Tuple_Agree_eq attrlist attr_eq_dec tup tup' = false.
-Proof.
-  destruct attr_eq_dec.
-  induction attrlist; unfold tupleAgree in *; simpl in *; simpl;
-  intuition;
-  unfold Tuple_Agree_eq in *; simpl in *; intuition;
-  find_if_inside; simpl; subst; eauto.
-  try (eapply IHattrlist; intros; eapply H).
-  intros; intuition; subst; auto.
-  eapply IHattrlist; intros; eauto.
-Qed.
-
-Definition Tuple_Agree_dec h attrlist
-           (attr_eq_dec : List_Query_eq (map (Domain h) attrlist)) (tup tup' : @Tuple h)
-: {tupleAgree tup tup' attrlist} + {~ tupleAgree tup tup' attrlist}.
-Proof.
-  case_eq (Tuple_Agree_eq attrlist attr_eq_dec tup tup').
-  left; eapply Tuple_Agree_eq_dec; eauto.
-  right; eapply Tuple_Agree_eq_dec'; eauto.
-Defined.
+  Definition Tuple_Agree_dec h attrlist
+             (attr_eq_dec : List_Query_eq (map (Domain h) attrlist)) (tup tup' : @Tuple h)
+    : {tupleAgree tup tup' attrlist} + {~ tupleAgree tup tup' attrlist}.
+  Proof.
+    case_eq (Tuple_Agree_eq attrlist attr_eq_dec tup tup').
+    left; eapply Tuple_Agree_eq_dec; eauto.
+    right; eapply Tuple_Agree_eq_dec'; eauto.
+  Defined.
 
 
   Lemma tupleAgree_sym :
@@ -99,516 +89,16 @@ Defined.
     split; intros; rewrite H; eauto.
   Qed.
 
-  Lemma refine_Iterate_Ensemble {A : Set}
-        (A_eq_dec : forall a a' : A, {a = a'} + {a <> a'})
-  : forall (As : list string)
-           (P : Ensemble (BoundedIndex As)),
-      refine {b | decides b (forall idx : BoundedIndex As, P idx)}
-             {b | decides b (@Iterate_Ensemble_BoundedIndex As P)}.
-  Proof.
-    intros; eapply refine_pick_pick.
-    intros; destruct x; simpl in *.
-    intros; eapply Iterate_Ensemble_equiv' with (Visited := []);
-    eauto using string_dec.
-    destruct n; simpl; intros; discriminate.
-    unfold not; intros; apply H.
-    apply Iterate_Ensemble_equiv'';
-      auto using string_dec.
-  Qed.
-
-  Lemma refine_Iterate_Ensemble_filter {A : Set}
-        (A_eq_dec : forall a a' : A, {a = a'} + {a <> a'})
-  : forall (As : list string)
-           (P : Ensemble (BoundedIndex As))
-           (filter : Ensemble nat)
-           (filter_dec : DecideableEnsemble filter),
-      refine {b | decides b (forall idx : BoundedIndex As,
-                               filter (ibound idx) -> P idx)}
-             {b | decides b (@Iterate_Ensemble_BoundedIndex_filter
-                               As (@dec _ _ filter_dec) P )}.
-  Proof.
-    intros; eapply refine_pick_pick.
-    intros; destruct x; simpl in *.
-    intros; eapply Iterate_Ensemble_equiv_filter' with (Visited := []);
-    eauto using string_dec.
-    destruct n; simpl; intros; discriminate.
-    unfold not; intros; apply H.
-    apply Iterate_Ensemble_equiv_filter''; auto using string_dec.
-  Qed.
-
-  Lemma refine_decides_Equiv_Ensemble {A : Set}
-        (A_eq_dec : forall a a' : A, {a = a'} + {a <> a'})
-  : forall (As : list string)
-           (P P' : Ensemble (BoundedIndex As))
-           (equiv_P'_P : (forall idx, P idx) <-> (forall idx', P' idx')),
-      refine {b | decides b (forall idx : BoundedIndex As, P idx)}
-             {b | decides b (forall idx : BoundedIndex As, P' idx)}.
-  Proof.
-    intros * equiv_P'_P v Comp_v.
-     computes_to_inv; computes_to_constructor; destruct v; simpl in *.
-    intros; eapply equiv_P'_P; eauto.
-    unfold not; intros; eapply Comp_v; eapply equiv_P'_P; eauto.
-  Qed.
-
-  Corollary Iterate_Ensemble_filter_neq {A : Set}
-        (A_eq_dec : forall a a' : A, {a = a'} + {a <> a'})
-  : forall (As : list string)
-           (P : Ensemble (BoundedIndex As))
-           (Ridx : BoundedIndex As),
-    (forall idx : BoundedIndex As, idx <> Ridx -> P idx)
-    <-> (@Iterate_Ensemble_BoundedIndex_filter
-           As (fun idx =>
-                 if (eq_nat_dec (ibound Ridx) idx)
-                 then false else true) P ).
-  Proof.
-    intros.
-    assert (forall a : nat,
-              (if eq_nat_dec (ibound Ridx) a then false else true) = true
-              <-> a <> ibound Ridx)
-      as filter_dec'
-      by (intros; find_if_inside; try rewrite e; intuition).
-    assert ((forall idx : BoundedIndex As, idx <> Ridx -> P idx)
-            <-> (forall idx  : BoundedIndex As,
-                   ibound idx <> ibound Ridx -> P idx)).
-    { split; intros; eauto.
-      apply H; destruct idx as [idx [n nth_n] ];
-      destruct Ridx as [Ridx [n' nth_n'] ]; simpl in *.
-      unfold not; intros; apply H0; injection H1; auto.
-      apply H; unfold not; intros; apply H0.
-      destruct idx as [idx [n nth_n] ];
-        destruct Ridx as [Ridx [n' nth_n'] ]; simpl in *.
-      clear H0; revert nth_n; rewrite H1; intros.
-      assert (Ridx = idx) by
-          (rewrite nth_n' in nth_n; congruence).
-      revert nth_n' nth_n; rewrite H0.
-      intros; repeat f_equal.
-      apply (eq_proofs_unicity_Opt_A string_dec).
-    }
-    rewrite H.
-    split; intros.
-    - eapply Iterate_Ensemble_equiv_filter'' with
-      (filter := fun idx => idx <> ibound Ridx)
-        (filter_dec := {|dec_decides_P := filter_dec' |}); eauto.
-      apply string_dec.
-    - eapply Iterate_Ensemble_equiv_filter'  with
-      (Visited := [])
-      (filter := fun idx => idx <> ibound Ridx)
-        (filter_dec := {|dec_decides_P := filter_dec' |});
-      unfold dec; eauto using string_dec.
-      intros; destruct n; simpl in *; discriminate.
-  Qed.
-
-  Lemma refine_Iterate_Equiv_Ensemble {A : Set}
-        (A_eq_dec : forall a a' : A, {a = a'} + {a <> a'})
-  : forall (As As' : list string)
-           (P : Ensemble (BoundedIndex As))
-           (P' : Ensemble (BoundedIndex As'))
-           (equiv_P'_P : (forall idx, P idx) <-> (forall idx', P' idx')),
-      refine {b | decides b (forall idx : BoundedIndex As, P idx)}
-             {b | decides b (@Iterate_Ensemble_BoundedIndex As' P')}.
-  Proof.
-    intros; setoid_rewrite refine_Iterate_Ensemble; try eassumption.
-    intros v Comp_v.
-     computes_to_inv; computes_to_constructor; destruct v; simpl in *.
-    apply Iterate_Ensemble_equiv'' with (Visited := []);
-      eauto using string_dec; simpl.
-    apply equiv_P'_P; intros;
-    apply Iterate_Ensemble_equiv' with (Visited := []);
-    eauto using string_dec; simpl.
-    destruct n; simpl; intros; discriminate.
-    unfold not; intros; apply Comp_v.
-    apply Iterate_Ensemble_equiv'';
-      auto using string_dec.
-    apply equiv_P'_P;
-    apply Iterate_Ensemble_equiv' with (Visited := []);
-    eauto using string_dec; simpl.
-    destruct n; simpl; intros; discriminate.
-  Qed.
-
-  (* So that things play nicely with setoid rewriting *)
-  Definition If_Then_Else {A}  (b : bool) (t e : A)
-    := if b then t else e.
-
-  Lemma refine_trivial_if_then_else :
-    forall x,
-      refine
-        (If_Then_Else x (ret true) (ret false))
-        (ret x).
-  Proof.
-    destruct x; reflexivity.
-  Qed.
-
-  Program Fixpoint Iterate_Decide_Comp' (A : Set)
-          (Remaining Visited : list A)
-          (P : Ensemble (BoundedIndex (Visited ++ Remaining)))
-          {struct Remaining }
-  : Comp bool :=
-    match Remaining with
-      | nil => ret true
-      | cons a Remaining' =>
-        Bind {b' |
-              decides b' (P {| bindex := a;
-                               indexb := {| ibound := List.length Visited;
-                                            boundi := _ |} |})}%comp
-             (fun b' =>
-                If_Then_Else b'
-                             (Iterate_Decide_Comp' _ Remaining' (Visited ++ [a]) _)
-                             (ret false))
-    end.
-  Next Obligation.
-    clear P; induction Visited; simpl; auto.
-  Defined.
-  Next Obligation.
-    exact (Ensemble_BoundedIndex_app_comm_cons _ _ _ P).
-  Defined.
-
-  Lemma refine_Iterate_Decided_Ensemble' {A : Set}
-        (A_eq_dec : forall a a' : A, {a = a'} + {a <> a'})
-  : forall (Remaining Visited : list A)
-           (P : Ensemble (BoundedIndex (Visited ++ Remaining))),
-      refine {b | decides b (Iterate_Ensemble_BoundedIndex' Visited Remaining P)}
-                  (Iterate_Decide_Comp' _ Remaining Visited P).
-  Proof.
-    induction Remaining; simpl; intros.
-    - computes_to_econstructor;  computes_to_inv; subst; simpl; auto.
-    - computes_to_econstructor; computes_to_inv; destruct_ex;
-      split_and;  computes_to_inv; subst.
-      destruct v0; simpl in *.
-      { destruct v; simpl in *; intuition; intros; eauto.
-        - generalize (IHRemaining (Visited ++ [a]) _ _ H').
-          intros;  computes_to_inv; simpl in *; eauto.
-        - generalize (IHRemaining (Visited ++ [a]) _ _ H').
-          intros;  computes_to_inv; simpl in *; eauto.
-      }
-      {  computes_to_inv; subst; simpl; intuition. }
-  Qed.
-
-  Definition Iterate_Decide_Comp
-          (Bound : list string)
-          (P : Ensemble (BoundedIndex Bound))
-  : Comp bool :=
-    Iterate_Decide_Comp' _ Bound [] P.
-
-  Definition Iterate_Decide_Comp_BoundedIndex
-  : forall (Bound : list string)
-           (P : Ensemble (BoundedIndex Bound)),
-      refine {b | decides b (forall Ridx', P Ridx')}
-             (Iterate_Decide_Comp _ P).
-  Proof.
-    intros.
-    setoid_rewrite refine_Iterate_Ensemble; auto using string_dec.
-    setoid_rewrite refine_Iterate_Decided_Ensemble'; auto using string_dec.
-    reflexivity.
-  Qed.
-
-  (* Variants for inserting additional assumptions into the
-   decision procedure. *)
-  Program Lemma refine_Iterate_Ensemble_Pre {A : Set}
-        (A_eq_dec : forall a a' : A, {a = a'} + {a <> a'})
-  : forall (As : list string)
-           (P : Ensemble (BoundedIndex As))
-           (Q : Prop),
-      refine {b | Q -> decides b (forall idx : BoundedIndex As, P idx)}
-             {b | Q -> decides b (@Iterate_Ensemble_BoundedIndex As P)}.
-  Proof.
-    intros; eapply refine_pick_pick.
-    intros; destruct x; simpl in *; apply H in H0.
-    intros; eapply Iterate_Ensemble_equiv' with (Visited := []);
-    eauto using string_dec.
-    destruct n; simpl; intros; discriminate.
-    unfold not; intros; apply H0.
-    apply Iterate_Ensemble_equiv'';
-      auto using string_dec.
-  Qed.
-
-  Program Fixpoint Iterate_Decide_Comp'_Pre (A : Set)
-          (Remaining Visited : list A)
-          (P : Ensemble (BoundedIndex (Visited ++ Remaining)))
-          (Q : Prop)
-          {struct Remaining }
-  : Comp bool :=
-    match Remaining with
-      | nil => ret true
-      | cons a Remaining' =>
-        Bind {b' | Q ->
-              decides b' (P {| bindex := a;
-                               indexb := {| ibound := List.length Visited;
-                                            boundi := _ |} |})}%comp
-             (fun b' =>
-                If_Then_Else b'
-                             (Iterate_Decide_Comp'_Pre _ Remaining' (Visited ++ [a]) _ Q)
-                             (ret false))
-    end.
-  Next Obligation.
-    clear P; induction Visited; simpl; auto.
-  Defined.
-  Next Obligation.
-    exact (Ensemble_BoundedIndex_app_comm_cons _ _ _ P).
-  Defined.
-
-  Lemma refine_Iterate_Decided_Ensemble'_Pre {A : Set}
-        (A_eq_dec : forall a a' : A, {a = a'} + {a <> a'})
-  : forall (Remaining Visited : list A)
-           (P : Ensemble (BoundedIndex (Visited ++ Remaining)))
-           (Q : Prop),
-      refine {b | Q -> decides b (Iterate_Ensemble_BoundedIndex' Visited Remaining P)}
-             (Iterate_Decide_Comp'_Pre _ Remaining Visited P Q).
-  Proof.
-    induction Remaining; simpl; intros.
-    - computes_to_econstructor;  computes_to_inv; subst; simpl; auto.
-    - computes_to_econstructor; computes_to_inv; destruct_ex;
-      split_and;  computes_to_inv; subst.
-      destruct v0; simpl in *.
-      {  destruct v; simpl in *; intuition; intros; eauto.
-         - generalize (IHRemaining (Visited ++ [a]) _ _ _ H').
-           intros;  computes_to_inv; simpl in *; eauto.
-         - generalize (IHRemaining (Visited ++ [a]) _ _ _ H').
-           intros;  computes_to_inv; simpl in *; eauto.
-           eapply H; eauto.
-      }
-      {  computes_to_inv; subst; simpl; intuition. }
-  Qed.
-
-  Definition Iterate_Decide_Comp_Pre
-          (Bound : list string)
-          (P : Ensemble (BoundedIndex Bound))
-          (Q : Prop)
-  : Comp bool :=
-    Iterate_Decide_Comp'_Pre _ Bound [] P Q.
-
-  Definition Iterate_Decide_Comp_BoundedIndex_Pre
-  : forall (Bound : list string)
-           (P : Ensemble (BoundedIndex Bound))
-           (Q : Prop),
-      refine {b | Q -> decides b (forall Ridx', P Ridx')}
-             (Iterate_Decide_Comp_Pre _ P Q).
-  Proof.
-    intros.
-    setoid_rewrite refine_Iterate_Ensemble_Pre; auto using string_dec.
-    setoid_rewrite refine_Iterate_Decided_Ensemble'_Pre; auto using string_dec.
-    reflexivity.
-  Qed.
-
-  Lemma decides_True :
-    refine {b | decides b True}%comp
-           (ret true).
-  Proof.
-    computes_to_econstructor;  computes_to_inv; subst; simpl; auto.
-  Qed.
-
-  Lemma decides_True_Pre (Q : Prop) :
-    refine {b | Q -> decides b True}%comp
-           (ret true).
-  Proof.
-    computes_to_econstructor;  computes_to_inv; subst; simpl; auto.
-  Qed.
-
-  Lemma decides_2_True (A : Type) (B : A -> Type) :
-    refine {b' | decides b' (forall a : A, B a -> True)}%comp
-           (ret true).
-  Proof.
-    computes_to_econstructor;  computes_to_inv; subst; simpl; auto.
-  Qed.
-
-  Lemma decides_3_True (A B : Type) (C : B -> Type) :
-    refine {b' | decides b' (A -> forall b : B, C b -> True)}%comp
-           (ret true).
-  Proof.
-    computes_to_econstructor;  computes_to_inv; subst; simpl; auto.
-  Qed.
-
-  Lemma decides_neq (A : Type) (B : Prop) (a : A) :
-    refine {b' | decides b' (a <> a -> B)}%comp
-           (ret true).
-  Proof.
-    computes_to_econstructor;  computes_to_inv; subst; simpl; auto.
-    congruence.
-  Qed.
-
-  Definition Ensemble_opt_BoundedIndex_app_comm_cons {A : Set}
-    (a : A)
-    (As As' : list A)
-    (P : BoundedIndex (As ++ a :: As') -> option Prop)
-  : BoundedIndex ((As ++ [a]) ++ As') -> option Prop.
-    rewrite app_comm_cons' in P; exact P.
-  Defined.
-
-  Program Fixpoint Iterate_Decide_Comp_opt' (A : Set)
-          (Remaining Visited : list A)
-          (P : BoundedIndex (Visited ++ Remaining) -> option Prop )
-          {struct Remaining }
-  : Comp bool :=
-    match Remaining with
-      | nil => ret true
-      | cons a Remaining' =>
-        match (P {| bindex := a;
-                    indexb := {| ibound := List.length Visited;
-                                 boundi := _ |} |}) with
-          | Some P' => b' <- {b' | decides b' P'};
-                      If_Then_Else b'
-                                   (Iterate_Decide_Comp_opt' _ Remaining' (Visited ++ [a])
-                                                             (Ensemble_opt_BoundedIndex_app_comm_cons _ _ _ P))
-                                   (ret false)
-          | None => (Iterate_Decide_Comp_opt' _ Remaining' (Visited ++ [a])
-                                              (Ensemble_opt_BoundedIndex_app_comm_cons _ _ _ P))
-        end
-    end%comp.
-  Next Obligation.
-    clear P; induction Visited; simpl; auto.
-  Defined.
-
-  Lemma refine_Iterate_Decide_Comp'
-        {A : Set}
-        (A_eq_dec : forall a a' : A, {a = a'} + {a <> a'})
-  : forall (Remaining Visited : list A)
-           (P : BoundedIndex (Visited ++ Remaining)
-                -> option Prop),
-      refine (@Iterate_Decide_Comp' _ Remaining Visited (fun idx => match P idx with
-                                                                      | Some P' => P'
-                                                                      | None => True
-                                                                    end))
-             (@Iterate_Decide_Comp_opt' _ Remaining Visited P).
-    induction Remaining; simpl; intros.
-    - reflexivity.
-    - destruct (P ``(a)).
-      + f_equiv; unfold pointwise_relation; intros.
-        destruct a0; simpl; try reflexivity.
-        setoid_rewrite <- IHRemaining; f_equiv.
-        unfold Ensemble_BoundedIndex_app_comm_cons,
-        Ensemble_opt_BoundedIndex_app_comm_cons; simpl.
-        destruct (app_comm_cons' a Visited Remaining); simpl.
-        reflexivity.
-      + rewrite decides_True; simplify with monad laws; simpl.
-        setoid_rewrite <- IHRemaining; f_equiv.
-        unfold Ensemble_BoundedIndex_app_comm_cons,
-        Ensemble_opt_BoundedIndex_app_comm_cons; simpl.
-        destruct (app_comm_cons' a Visited Remaining); simpl.
-        reflexivity.
-  Qed.
-
-  Lemma refine_Iterate_Decide_Comp
-  : forall (Bound : list string)
-           (P : BoundedIndex Bound -> option Prop),
-      refine (@Iterate_Decide_Comp _ (fun idx => match P idx with
-                                                 | Some P' => P'
-                                                 | None => True
-                                               end))
-             (@Iterate_Decide_Comp_opt' _ Bound [] P).
-  Proof.
-    intros; unfold Iterate_Decide_Comp;
-    rewrite refine_Iterate_Decide_Comp'.
-    reflexivity.
-    apply string_dec.
-  Qed.
-
-  Program Fixpoint Iterate_Decide_Comp_opt'_Pre (A : Set)
-          (Remaining Visited : list A)
-          (P : BoundedIndex (Visited ++ Remaining) -> option Prop)
-          (Q : Prop)
-          {struct Remaining }
-  : Comp bool :=
-    match Remaining with
-      | nil => ret true
-      | cons a Remaining' =>
-        match (P {| bindex := a;
-                    indexb := {| ibound := List.length Visited;
-                                 boundi := _ |} |}) with
-          | Some P' => b' <- {b' | Q -> decides b' P'};
-                      If_Then_Else b'
-                                   (Iterate_Decide_Comp_opt'_Pre _ Remaining' (Visited ++ [a])
-                                                             (Ensemble_opt_BoundedIndex_app_comm_cons _ _ _ P) Q)
-                                   (ret false)
-          | None => (Iterate_Decide_Comp_opt'_Pre _ Remaining' (Visited ++ [a])
-                                              (Ensemble_opt_BoundedIndex_app_comm_cons _ _ _ P) Q)
-        end
-    end%comp.
-  Next Obligation.
-    clear P; induction Visited; simpl; auto.
-  Defined.
-
-  Lemma refine_Iterate_Decide_Comp'_Pre
-        {A : Set}
-        (A_eq_dec : forall a a' : A, {a = a'} + {a <> a'})
-  : forall (Remaining Visited : list A)
-           (P : BoundedIndex (Visited ++ Remaining) -> option Prop)
-           (Q : Prop),
-      refine (@Iterate_Decide_Comp'_Pre _ Remaining Visited
-                                        (fun idx => match P idx with
-                                                      | Some P' => P'
-                                                      | None => True
-                                                    end) Q)
-             (@Iterate_Decide_Comp_opt'_Pre _ Remaining Visited P Q).
-  Proof.
-    induction Remaining; simpl; intros.
-    - reflexivity.
-    - destruct (P ``(a)).
-      + f_equiv; unfold pointwise_relation; intros.
-        destruct a0; simpl; try reflexivity.
-        setoid_rewrite <- IHRemaining; f_equiv.
-        unfold Ensemble_BoundedIndex_app_comm_cons,
-        Ensemble_opt_BoundedIndex_app_comm_cons; simpl.
-        destruct (app_comm_cons' a Visited Remaining); simpl.
-        reflexivity.
-      + rewrite decides_True_Pre; simplify with monad laws; simpl.
-        setoid_rewrite <- IHRemaining; f_equiv.
-        unfold Ensemble_BoundedIndex_app_comm_cons,
-        Ensemble_opt_BoundedIndex_app_comm_cons; simpl.
-        destruct (app_comm_cons' a Visited Remaining); simpl.
-        reflexivity.
-  Qed.
-
-  Lemma refine_Iterate_Decide_Comp_Pre
-  : forall (Bound : list string)
-           (P : BoundedIndex Bound -> option Prop)
-           (Q : Prop),
-      refine (@Iterate_Decide_Comp_Pre _ (fun idx => match P idx with
-                                                 | Some P' => P'
-                                                 | None => True
-                                               end) Q)
-             (@Iterate_Decide_Comp_opt'_Pre _ Bound [] P Q).
-  Proof.
-    intros; unfold Iterate_Decide_Comp_Pre;
-    rewrite refine_Iterate_Decide_Comp'_Pre.
-    reflexivity.
-    apply string_dec.
-  Qed.
-
-  Lemma refine_Iterate_Decide_Comp_equiv_Pre
-        (Q Q' : Prop)
-        {A : Set}
-        (A_eq_dec : forall a a' : A, {a = a'} + {a <> a'})
-  : forall (Remaining Visited : list A)
-           (P P' : Ensemble (BoundedIndex (Visited ++ Remaining))),
-      (forall idx, P idx -> P' idx)
-      -> (forall idx, ~ P idx -> ~ P' idx)
-      -> (Q -> Q')
-      -> refine (@Iterate_Decide_Comp'_Pre _ Remaining Visited P' Q)
-                (@Iterate_Decide_Comp'_Pre _ Remaining Visited P Q').
-  Proof.
-    induction Remaining; simpl; intros.
-    - reflexivity.
-    - f_equiv.
-      + unfold refine; intros;  computes_to_inv; subst;
-      computes_to_econstructor; destruct v; simpl in *; eauto.
-      + unfold pointwise_relation; intros b; destruct b; simpl.
-        apply IHRemaining; eauto.
-        unfold Ensemble_BoundedIndex_app_comm_cons; simpl;
-        destruct (app_comm_cons' a Visited Remaining); simpl; eauto.
-        unfold Ensemble_BoundedIndex_app_comm_cons; simpl;
-        destruct (app_comm_cons' a Visited Remaining); simpl; eauto.
-        reflexivity.
-  Qed.
-
   (* Consequences of ith_replace_BoundIndex_neq and ith_replace_BoundIndex_eq on updates *)
 
   Lemma refine_SatisfiesAttributeConstraints_self
-  : forall qsSchema
-           (Ridx : @BoundedString (map relName (qschemaSchemas qsSchema)))
-           (tup : @Tuple (schemaHeading (QSGetNRelSchema qsSchema Ridx))),
+    : forall qsSchema
+             (Ridx : @BoundedString (map relName (qschemaSchemas qsSchema)))
+             (tup : @Tuple (schemaHeading (QSGetNRelSchema qsSchema Ridx))),
       refine {b | decides b (SatisfiesAttributeConstraints Ridx tup )}
              match (attrConstraints (QSGetNRelSchema qsSchema Ridx)) with
-                 Some Constr => {b | decides b (Constr tup) }
-               | None => ret true
+               Some Constr => {b | decides b (Constr tup) }
+             | None => ret true
              end.
   Proof.
     unfold SatisfiesAttributeConstraints.
@@ -618,13 +108,13 @@ Defined.
   Qed.
 
   Lemma refine_SatisfiesTupleConstraints_self
-  : forall qsSchema
-           (Ridx : @BoundedString (map relName (qschemaSchemas qsSchema)))
-           (tup tup' : @Tuple (schemaHeading (QSGetNRelSchema qsSchema Ridx))),
+    : forall qsSchema
+             (Ridx : @BoundedString (map relName (qschemaSchemas qsSchema)))
+             (tup tup' : @Tuple (schemaHeading (QSGetNRelSchema qsSchema Ridx))),
       refine {b | decides b (SatisfiesTupleConstraints Ridx tup tup')}
              match (tupleConstraints (QSGetNRelSchema qsSchema Ridx)) with
-                 Some Constr => {b | decides b (Constr tup tup') }
-               | None => ret true
+               Some Constr => {b | decides b (Constr tup tup') }
+             | None => ret true
              end.
   Proof.
     unfold SatisfiesTupleConstraints.
@@ -634,23 +124,23 @@ Defined.
   Qed.
 
   Lemma refine_SatisfiesTupleConstraints
-  : forall qsSchema qs
-           (Ridx : @BoundedString (map relName (qschemaSchemas qsSchema)))
-           (tup : @Tuple (schemaHeading (QSGetNRelSchema qsSchema Ridx))),
+    : forall qsSchema qs
+             (Ridx : @BoundedString (map relName (qschemaSchemas qsSchema)))
+             (tup : @Tuple (schemaHeading (QSGetNRelSchema qsSchema Ridx))),
       refine {b | decides
                     b
                     (forall tup',
-                       GetUnConstrRelation qs Ridx tup'
-                       -> SatisfiesTupleConstraints
-                            Ridx
-                            tup
-                            (indexedElement tup'))}
+                        GetUnConstrRelation qs Ridx tup'
+                        -> SatisfiesTupleConstraints
+                             Ridx
+                             tup
+                             (indexedElement tup'))}
              match (tupleConstraints (QSGetNRelSchema qsSchema Ridx)) with
-                 Some Constr =>
-                 {b | decides b (forall tup',
-                                   GetUnConstrRelation qs Ridx tup'
-                                   -> Constr tup (indexedElement tup'))}
-               | None => ret true
+               Some Constr =>
+               {b | decides b (forall tup',
+                                  GetUnConstrRelation qs Ridx tup'
+                                  -> Constr tup (indexedElement tup'))}
+             | None => ret true
              end.
   Proof.
     unfold SatisfiesTupleConstraints.
@@ -661,19 +151,19 @@ Defined.
   Qed.
 
   Lemma refine_SatisfiesTupleConstraints'
-  : forall qsSchema qs
-           (Ridx : @BoundedString (map relName (qschemaSchemas qsSchema)))
-           (tup : @Tuple (schemaHeading (QSGetNRelSchema qsSchema Ridx))),
+    : forall qsSchema qs
+             (Ridx : @BoundedString (map relName (qschemaSchemas qsSchema)))
+             (tup : @Tuple (schemaHeading (QSGetNRelSchema qsSchema Ridx))),
       refine {b | decides b
                           (forall tup',
-                             GetUnConstrRelation qs Ridx tup'
-                             -> SatisfiesTupleConstraints Ridx (indexedElement tup') tup)}
+                              GetUnConstrRelation qs Ridx tup'
+                              -> SatisfiesTupleConstraints Ridx (indexedElement tup') tup)}
              match (tupleConstraints (QSGetNRelSchema qsSchema Ridx)) with
-                 Some Constr =>
-                 {b | decides b (forall tup',
-                                   GetUnConstrRelation qs Ridx tup'
-                                   -> Constr (indexedElement tup') tup)}
-               | None => ret true
+               Some Constr =>
+               {b | decides b (forall tup',
+                                  GetUnConstrRelation qs Ridx tup'
+                                  -> Constr (indexedElement tup') tup)}
+             | None => ret true
              end.
   Proof.
     unfold SatisfiesTupleConstraints.
@@ -684,9 +174,9 @@ Defined.
   Qed.
 
   Lemma refine_SatisfiesCrossConstraints
-  : forall qsSchema qs
-           (Ridx : @BoundedString (map relName (qschemaSchemas qsSchema)))
-           (tup : @Tuple (schemaHeading (QSGetNRelSchema qsSchema Ridx))),
+    : forall qsSchema qs
+             (Ridx : @BoundedString (map relName (qschemaSchemas qsSchema)))
+             (tup : @Tuple (schemaHeading (QSGetNRelSchema qsSchema Ridx))),
       refine
         (@Iterate_Decide_Comp _
                               (fun Ridx' =>
@@ -696,9 +186,9 @@ Defined.
         (@Iterate_Decide_Comp_opt' _ _ []
                                    (fun Ridx' =>
                                       match (BuildQueryStructureConstraints qsSchema Ridx Ridx') with
-                                        | Some CrossConstr =>
-                                          Some (CrossConstr tup (GetUnConstrRelation qs Ridx'))
-                                        | None => None
+                                      | Some CrossConstr =>
+                                        Some (CrossConstr tup (GetUnConstrRelation qs Ridx'))
+                                      | None => None
                                       end)) .
   Proof.
     intros.
@@ -708,35 +198,11 @@ Defined.
     destruct BuildQueryStructureConstraints; reflexivity.
   Qed.
 
-  Lemma refine_Iterate_Decide_Comp_equiv
-        {A : Set}
-        (A_eq_dec : forall a a' : A, {a = a'} + {a <> a'})
-  : forall (Remaining Visited : list A)
-           (P P' : Ensemble (BoundedIndex (Visited ++ Remaining))),
-      (forall idx, P idx -> P' idx) ->
-      (forall idx, ~ P idx -> ~ P' idx) ->
-      refine (@Iterate_Decide_Comp' _ Remaining Visited P')
-             (@Iterate_Decide_Comp' _ Remaining Visited P).
-  Proof.
-    induction Remaining; simpl; intros.
-    - reflexivity.
-    - f_equiv.
-      + unfold refine; intros;  computes_to_inv; subst;
-        computes_to_econstructor; destruct v; simpl in *; eauto.
-      + unfold pointwise_relation; intros b; destruct b; simpl.
-        apply IHRemaining.
-        unfold Ensemble_BoundedIndex_app_comm_cons; simpl;
-        destruct (app_comm_cons' a Visited Remaining); simpl; eauto.
-        unfold Ensemble_BoundedIndex_app_comm_cons; simpl;
-        destruct (app_comm_cons' a Visited Remaining); simpl; eauto.
-        reflexivity.
-  Qed.
-
   Lemma tupleAgree_refl :
-  forall (h : Heading)
-         (tup : @Tuple h)
-         (attrlist : list (Attributes h)),
-    tupleAgree tup tup attrlist.
+    forall (h : Heading)
+           (tup : @Tuple h)
+           (attrlist : list (Attributes h)),
+      tupleAgree tup tup attrlist.
   Proof.
     unfold tupleAgree; auto.
   Qed.
@@ -755,22 +221,22 @@ Defined.
   Qed.
 
   Lemma refine_SatisfiesCrossConstraints_Pre (Q : Prop)
-  : forall qsSchema qs
-           (Ridx : @BoundedString (map relName (qschemaSchemas qsSchema)))
-           (tup : @Tuple (schemaHeading (QSGetNRelSchema qsSchema Ridx))),
+    : forall qsSchema qs
+             (Ridx : @BoundedString (map relName (qschemaSchemas qsSchema)))
+             (tup : @Tuple (schemaHeading (QSGetNRelSchema qsSchema Ridx))),
       refine
         (@Iterate_Decide_Comp_Pre _
-                              (fun Ridx' =>
-                                 SatisfiesCrossRelationConstraints
-                                   Ridx Ridx' tup
-                                   (GetUnConstrRelation qs Ridx')) Q)
+                                  (fun Ridx' =>
+                                     SatisfiesCrossRelationConstraints
+                                       Ridx Ridx' tup
+                                       (GetUnConstrRelation qs Ridx')) Q)
         (@Iterate_Decide_Comp_opt'_Pre _ _ []
-                                   (fun Ridx' =>
-                                      match (BuildQueryStructureConstraints qsSchema Ridx Ridx') with
-                                        | Some CrossConstr =>
-                                          Some (CrossConstr tup (GetUnConstrRelation qs Ridx'))
-                                        | None => None
-                                      end) Q) .
+                                       (fun Ridx' =>
+                                          match (BuildQueryStructureConstraints qsSchema Ridx Ridx') with
+                                          | Some CrossConstr =>
+                                            Some (CrossConstr tup (GetUnConstrRelation qs Ridx'))
+                                          | None => None
+                                          end) Q) .
   Proof.
     intros.
     setoid_rewrite <- refine_Iterate_Decide_Comp_Pre.
@@ -780,19 +246,19 @@ Defined.
   Qed.
 
   Lemma DeletePrimaryKeysOK {qsSchema}
-  : forall (qs : UnConstrQueryStructure qsSchema)
-           (Ridx : @BoundedString (map relName (qschemaSchemas qsSchema)))
-           DeletedTuples
-           attrlist1 attrlist2,
+    : forall (qs : UnConstrQueryStructure qsSchema)
+             (Ridx : @BoundedString (map relName (qschemaSchemas qsSchema)))
+             DeletedTuples
+             attrlist1 attrlist2,
       refine {b | (forall tup tup',
-                     elementIndex tup <> elementIndex tup'
-                     -> GetUnConstrRelation qs Ridx tup
-                     -> GetUnConstrRelation qs Ridx tup'
-                     -> (FunctionalDependency_P attrlist1 attrlist2 (indexedElement tup) (indexedElement tup')))
+                      elementIndex tup <> elementIndex tup'
+                      -> GetUnConstrRelation qs Ridx tup
+                      -> GetUnConstrRelation qs Ridx tup'
+                      -> (FunctionalDependency_P attrlist1 attrlist2 (indexedElement tup) (indexedElement tup')))
                   -> decides b (Mutate.MutationPreservesTupleConstraints
                                   (EnsembleDelete (GetUnConstrRelation qs Ridx) DeletedTuples)
                                   (FunctionalDependency_P attrlist1 attrlist2)
-                               )}
+             )}
              (ret true).
   Proof.
     unfold Mutate.MutationPreservesTupleConstraints, FunctionalDependency_P;
@@ -810,14 +276,14 @@ Defined.
            (bod : Comp (list B)),
     forall a,
       refine
-             (if (dec a) then
-                bod
-              else
-                (ret []))
-             (Where (P a) bod)%QuerySpec.
+        (if (dec a) then
+           bod
+         else
+           (ret []))
+        (Where (P a) bod)%QuerySpec.
   Proof.
     unfold refine, Query_Where; intros.
-     computes_to_inv; intuition.
+    computes_to_inv; intuition.
     caseEq (dec a).
     apply dec_decides_P in H; eauto.
     rewrite H1; eauto.
@@ -825,7 +291,7 @@ Defined.
   Qed.
 
   Lemma In_UnConstrQuery_In {qsSchema} {A}
-  : forall (qs : UnConstrQueryStructure qsSchema) Ridx bod results,
+    : forall (qs : UnConstrQueryStructure qsSchema) Ridx bod results,
       UnConstrQuery_In qs Ridx bod ↝ results
       -> forall (a : A), List.In a results ->
                          exists (tup' : IndexedTuple) results',
@@ -834,13 +300,13 @@ Defined.
                            /\ List.In a results'.
   Proof.
     unfold UnConstrQuery_In, QueryResultComp; intros;
-     computes_to_inv.
+    computes_to_inv.
     unfold UnIndexedEnsembleListEquivalence in *; destruct_ex; intuition; subst.
     rewrite map_map in H'.
     remember (GetUnConstrRelation qs Ridx); clear Hequ;
     revert u a results H0 H' H H3;
     induction x; simpl in *; intros;
-     computes_to_inv; subst.
+    computes_to_inv; subst.
     - simpl in H0; intuition.
     - apply in_app_or in H0; intuition.
       exists a v; intuition; try eapply H; eauto.
@@ -856,10 +322,10 @@ Defined.
   Qed.
 
   Lemma In_UnConstrQuery_In' {qsSchema} {A}
-  : forall (qs : UnConstrQueryStructure qsSchema) Ridx
-           (bod : Tuple -> Comp (list A))
-           results
-           (a : A) (tup' : IndexedTuple),
+    : forall (qs : UnConstrQueryStructure qsSchema) Ridx
+             (bod : Tuple -> Comp (list A))
+             results
+             (a : A) (tup' : IndexedTuple),
       Ensembles.In _ (GetUnConstrRelation qs Ridx) tup'
       -> (forall results', bod (indexedElement tup') ↝ results'
                            -> List.In a results')
@@ -867,54 +333,54 @@ Defined.
       -> List.In a results.
   Proof.
     unfold UnConstrQuery_In, QueryResultComp, Ensembles.In; intros.
-     computes_to_inv.
+    computes_to_inv.
     unfold UnIndexedEnsembleListEquivalence in *; destruct_ex; intuition; subst.
     rewrite map_map in H1'.
     remember (GetUnConstrRelation qs Ridx); clear Hequ;
     revert u a results H H0 H1 H1' H4;
     induction x; simpl in *; intros;
-     computes_to_inv; subst.
+    computes_to_inv; subst.
     - simpl in *; intuition; eapply H1; eauto.
     - apply H1 in H; intuition; subst; apply in_or_app; eauto.
-    right; inversion H4; subst.
-    eapply (IHx (fun tup => tup <> a /\ u tup)); eauto.
-    intuition; subst; eauto.
-    apply H5; eauto using in_map.
-    apply H1; eauto.
-    unfold Ensembles.In; intuition; intros; eauto.
-    rewrite H1 in H7; intuition.
-    subst; eauto using in_map.
-    apply H1; eauto.
+      right; inversion H4; subst.
+      eapply (IHx (fun tup => tup <> a /\ u tup)); eauto.
+      intuition; subst; eauto.
+      apply H5; eauto using in_map.
+      apply H1; eauto.
+      unfold Ensembles.In; intuition; intros; eauto.
+      rewrite H1 in H7; intuition.
+      subst; eauto using in_map.
+      apply H1; eauto.
   Qed.
 
   Lemma DeleteForeignKeysCheck {qsSchema}
-  : forall (qs : UnConstrQueryStructure qsSchema)
-           (Ridx Ridx' : @BoundedString (map relName (qschemaSchemas qsSchema)))
-           (DeletedTuples : Ensemble (@Tuple (schemaHeading (QSGetNRelSchema _ Ridx))))
-           (Delete_dec : DecideableEnsemble DeletedTuples)
-           (attr : Attributes (schemaHeading (QSGetNRelSchema _ Ridx)))
-           (attr' : Attributes (schemaHeading (QSGetNRelSchema _ Ridx')))
-           (tupmap : Domain (schemaHeading (QSGetNRelSchema _ Ridx)) attr
-                     -> Domain (schemaHeading (QSGetNRelSchema _ Ridx')) attr')
-           (AgreeDelete : forall tup tup',
-                            tupleAgree tup tup' [attr] ->
-                            DeletedTuples tup ->
-                            DeletedTuples tup')
-           (attr_eq_dec : Query_eq (Domain (schemaHeading (QSGetNRelSchema _ Ridx)) attr))
-           (P : Prop)
-           (ForeignKey_P_P :
-              P -> (forall tup' : IndexedTuple,
-                        GetUnConstrRelation qs Ridx' tup' ->
-                        ForeignKey_P attr' attr tupmap (indexedElement tup')
-                                     (GetUnConstrRelation qs Ridx)))
-           (tup_map_inj : forall a a', tupmap a = tupmap a' -> a = a'),
+    : forall (qs : UnConstrQueryStructure qsSchema)
+             (Ridx Ridx' : @BoundedString (map relName (qschemaSchemas qsSchema)))
+             (DeletedTuples : Ensemble (@Tuple (schemaHeading (QSGetNRelSchema _ Ridx))))
+             (Delete_dec : DecideableEnsemble DeletedTuples)
+             (attr : Attributes (schemaHeading (QSGetNRelSchema _ Ridx)))
+             (attr' : Attributes (schemaHeading (QSGetNRelSchema _ Ridx')))
+             (tupmap : Domain (schemaHeading (QSGetNRelSchema _ Ridx)) attr
+                       -> Domain (schemaHeading (QSGetNRelSchema _ Ridx')) attr')
+             (AgreeDelete : forall tup tup',
+                 tupleAgree tup tup' [attr] ->
+                 DeletedTuples tup ->
+                 DeletedTuples tup')
+             (attr_eq_dec : Query_eq (Domain (schemaHeading (QSGetNRelSchema _ Ridx)) attr))
+             (P : Prop)
+             (ForeignKey_P_P :
+                P -> (forall tup' : IndexedTuple,
+                         GetUnConstrRelation qs Ridx' tup' ->
+                         ForeignKey_P attr' attr tupmap (indexedElement tup')
+                                      (GetUnConstrRelation qs Ridx)))
+             (tup_map_inj : forall a a', tupmap a = tupmap a' -> a = a'),
       refine {b' |
               P ->
-               decides b'
-                       (MutationPreservesCrossConstraints
-                          (GetUnConstrRelation qs Ridx')
-                          (EnsembleDelete (GetUnConstrRelation qs Ridx) DeletedTuples)
-                          (ForeignKey_P attr' attr tupmap))}
+              decides b'
+                      (MutationPreservesCrossConstraints
+                         (GetUnConstrRelation qs Ridx')
+                         (EnsembleDelete (GetUnConstrRelation qs Ridx) DeletedTuples)
+                         (ForeignKey_P attr' attr tupmap))}
              (x <- Count (For (UnConstrQuery_In
                                  qs Ridx'
                                  (fun tup' =>
@@ -922,11 +388,11 @@ Defined.
                                       qs Ridx
                                       (fun tup =>
                                          Where (DeletedTuples tup)
-                                         Where (tupmap (GetAttribute tup attr) = GetAttribute tup' attr')
-                                         Return ()))));
+                                               Where (tupmap (GetAttribute tup attr) = GetAttribute tup' attr')
+                                               Return ()))));
               ret (match x with
-                       0  => true
-                     | S _ => false
+                     0  => true
+                   | S _ => false
                    end)).
   Proof.
     simpl; unfold ForeignKey_P; intros.
@@ -978,8 +444,8 @@ Defined.
           [rewrite H17 in *; eauto | intuition ].
         * rewrite H16 in H11; simpl in *; eauto.
           intros;
-          unfold QSGetNRelSchema, GetNRelSchema in *; simpl in *;
-          rewrite <- H17 in H9; eauto.
+            unfold QSGetNRelSchema, GetNRelSchema in *; simpl in *;
+            rewrite <- H17 in H9; eauto.
       + rewrite H14 in H11; simpl in *; eauto.
         intros H'; apply dec_decides_P in H'; congruence.
       + eapply Permutation_in; symmetry in Comp_v'; simpl; eauto.
@@ -988,7 +454,7 @@ Defined.
   Qed.
 
   Lemma InsertForeignKeysCheck {qsSchema}
-  : forall
+    : forall
       (qs : UnConstrQueryStructure qsSchema)
       (Ridx Ridx' : @BoundedString (map relName (qschemaSchemas qsSchema)))
       (attr : Attributes (schemaHeading (QSGetNRelSchema _ Ridx)))
@@ -998,17 +464,17 @@ Defined.
       tup
       (ForeignKey_P_P :
          (forall tup' : IndexedTuple,
-            GetUnConstrRelation qs Ridx tup' ->
-            ForeignKey_P attr attr' tupmap (indexedElement tup')
-                         (GetUnConstrRelation qs Ridx'))),
+             GetUnConstrRelation qs Ridx tup' ->
+             ForeignKey_P attr attr' tupmap (indexedElement tup')
+                          (GetUnConstrRelation qs Ridx'))),
       Ridx <> Ridx'
       -> refine {b' |
                  decides b'
                          (forall tup',
-                            (GetUnConstrRelation qs Ridx) tup' ->
-                            ForeignKey_P attr attr' tupmap
-                                         (indexedElement tup')
-                                         (EnsembleInsert tup (GetUnConstrRelation qs Ridx')))}
+                             (GetUnConstrRelation qs Ridx) tup' ->
+                             ForeignKey_P attr attr' tupmap
+                                          (indexedElement tup')
+                                          (EnsembleInsert tup (GetUnConstrRelation qs Ridx')))}
                 (ret true).
   Proof.
     intros; apply refine_pick_val; simpl; intros.
@@ -1123,7 +589,7 @@ Proof.
 Qed.
 
 Lemma UnIndexedEnsembleListEquivalence_eqv {A}
-: forall ens l,
+  : forall ens l,
     @UnIndexedEnsembleListEquivalence A ens l ->
     exists l',
       EnsembleListEquivalence ens l' /\ l = map indexedElement l'.
@@ -1171,7 +637,7 @@ Lemma refine_constraint_check_into_query' :
          (Pick (fun (b : bool) =>
                   decides b
                           (exists tup2: @IndexedTuple _,
-                             (GetUnConstrRelation c tbl tup2 /\ P' tup2))))
+                              (GetUnConstrRelation c tbl tup2 /\ P' tup2))))
          (Bind
             (Count (For (UnConstrQuery_In c tbl (fun tup => Where (P tup) Return tup))))
             (fun count => ret (negb (beq_nat count 0)))).
@@ -1179,7 +645,7 @@ Proof.
   Local Transparent Count.
   unfold refine, Count, UnConstrQuery_In;
     intros * excl * P_iff_P' pick_comp ** .
-   computes_to_inv; subst.
+  computes_to_inv; subst.
 
   computes_to_constructor.
 
@@ -1197,24 +663,24 @@ Proof.
   apply decidable_excl; assumption.
 Qed.
 
-    Corollary refine_constraint_check_into_query :
-    forall {schm tbl} P (c : UnConstrQueryStructure schm)
-           (P_dec : DecideableEnsemble P),
-        refine
-          (Pick (fun (b : bool) =>
-                   decides b
-                           (exists tup2: @IndexedTuple _,
-                              (GetUnConstrRelation c tbl tup2 /\ P (indexedTuple tup2)))))
-          (Bind
-             (Count (For (UnConstrQuery_In c tbl (fun tup => Where (P tup) Return tup))))
-             (fun count => ret (negb (beq_nat count 0)))).
-    Proof.
+Corollary refine_constraint_check_into_query :
+  forall {schm tbl} P (c : UnConstrQueryStructure schm)
+         (P_dec : DecideableEnsemble P),
+    refine
+      (Pick (fun (b : bool) =>
+               decides b
+                       (exists tup2: @IndexedTuple _,
+                           (GetUnConstrRelation c tbl tup2 /\ P (indexedTuple tup2)))))
+      (Bind
+         (Count (For (UnConstrQuery_In c tbl (fun tup => Where (P tup) Return tup))))
+         (fun count => ret (negb (beq_nat count 0)))).
+Proof.
 
-      intros.
-      setoid_rewrite refine_constraint_check_into_query'; eauto.
-      reflexivity.
-      unfold Same_set, Included; intuition.
-    Qed.
+  intros.
+  setoid_rewrite refine_constraint_check_into_query'; eauto.
+  reflexivity.
+  unfold Same_set, Included; intuition.
+Qed.
 
 Definition refine_foreign_key_check_into_query {schm tbl} :=
   @refine_constraint_check_into_query schm tbl.
@@ -1223,26 +689,26 @@ Lemma refine_functional_dependency_check_into_query :
   forall {schm : QueryStructureSchema} {tbl} ref args1 args2 (c : UnConstrQueryStructure schm),
     DecideableEnsemble (fun x : Tuple => tupleAgree_computational ref x args1 /\
                                          ~ tupleAgree_computational ref x args2) ->
-      ((forall tup' : IndexedTuple,
-          GetUnConstrRelation c tbl tup'
-          -> FunctionalDependency_P args2 args1 ref (indexedElement tup'))
-       <-> (forall tup' : IndexedTuple,
-          ~ (GetUnConstrRelation c tbl tup'
-             /\ tupleAgree ref (indexedElement tup') args1
-             /\ ~ tupleAgree ref (indexedElement tup') args2))) ->
-      refine
-        (Pick (fun (b : bool) =>
-                 decides b
-                         (forall tup' : IndexedTuple,
-                            GetUnConstrRelation c tbl tup' ->
-                            FunctionalDependency_P args2 args1 ref (indexedElement tup'))))
-        (Bind (Count
-                 For (UnConstrQuery_In c tbl
-                                       (fun tup : Tuple =>
-                                          Where (tupleAgree_computational ref tup args1 /\
-                                                 ~ tupleAgree_computational ref tup args2)
-                                                Return tup)))
-              (fun count => ret (beq_nat count 0))).
+    ((forall tup' : IndexedTuple,
+         GetUnConstrRelation c tbl tup'
+         -> FunctionalDependency_P args2 args1 ref (indexedElement tup'))
+     <-> (forall tup' : IndexedTuple,
+             ~ (GetUnConstrRelation c tbl tup'
+                /\ tupleAgree ref (indexedElement tup') args1
+                /\ ~ tupleAgree ref (indexedElement tup') args2))) ->
+    refine
+      (Pick (fun (b : bool) =>
+               decides b
+                       (forall tup' : IndexedTuple,
+                           GetUnConstrRelation c tbl tup' ->
+                           FunctionalDependency_P args2 args1 ref (indexedElement tup'))))
+      (Bind (Count
+               For (UnConstrQuery_In c tbl
+                                     (fun tup : Tuple =>
+                                        Where (tupleAgree_computational ref tup args1 /\
+                                               ~ tupleAgree_computational ref tup args2)
+                                              Return tup)))
+            (fun count => ret (beq_nat count 0))).
 Proof.
   intros * is_dec ** .
 
@@ -1256,8 +722,8 @@ Proof.
   setoid_rewrite refine_decide_negation.
   setoid_rewrite tupleAgree_equivalence.
   setoid_rewrite (@refine_constraint_check_into_query _ _
-                    (fun (x: Tuple ) => tupleAgree_computational ref x args1 /\
-                                        ~ tupleAgree_computational ref x args2)); try assumption.
+                                                      (fun (x: Tuple ) => tupleAgree_computational ref x args1 /\
+                                                                          ~ tupleAgree_computational ref x args2)); try assumption.
 
   Opaque Query_For Count.
   simplify with monad laws.
@@ -1269,26 +735,26 @@ Lemma refine_functional_dependency_check_into_query' :
   forall {schm : QueryStructureSchema} {tbl} ref args1 args2 (c : UnConstrQueryStructure schm),
     DecideableEnsemble (fun x : Tuple => tupleAgree_computational x ref args1 /\
                                          ~ tupleAgree_computational x ref args2) ->
-      ((forall tup' : IndexedTuple,
-          GetUnConstrRelation c tbl tup'
-          -> FunctionalDependency_P args2 args1 (indexedElement tup') ref)
-       <-> (forall tup' : IndexedTuple,
-          ~ (GetUnConstrRelation c tbl tup'
-             /\ tupleAgree (indexedElement tup') ref args1
-             /\ ~ tupleAgree (indexedElement tup') ref args2))) ->
-      refine
-        (Pick (fun (b : bool) =>
-                 decides b
-                         (forall tup' : IndexedTuple,
-                            GetUnConstrRelation c tbl tup' ->
-                            FunctionalDependency_P args2 args1 (indexedElement tup') ref)))
-        (Bind (Count
-                 For (UnConstrQuery_In c tbl
-                                       (fun tup : Tuple =>
-                                          Where (tupleAgree_computational tup ref args1 /\
-                                                 ~ tupleAgree_computational tup ref args2)
-                                                Return tup)))
-              (fun count => ret (beq_nat count 0))).
+    ((forall tup' : IndexedTuple,
+         GetUnConstrRelation c tbl tup'
+         -> FunctionalDependency_P args2 args1 (indexedElement tup') ref)
+     <-> (forall tup' : IndexedTuple,
+             ~ (GetUnConstrRelation c tbl tup'
+                /\ tupleAgree (indexedElement tup') ref args1
+                /\ ~ tupleAgree (indexedElement tup') ref args2))) ->
+    refine
+      (Pick (fun (b : bool) =>
+               decides b
+                       (forall tup' : IndexedTuple,
+                           GetUnConstrRelation c tbl tup' ->
+                           FunctionalDependency_P args2 args1 (indexedElement tup') ref)))
+      (Bind (Count
+               For (UnConstrQuery_In c tbl
+                                     (fun tup : Tuple =>
+                                        Where (tupleAgree_computational tup ref args1 /\
+                                               ~ tupleAgree_computational tup ref args2)
+                                              Return tup)))
+            (fun count => ret (beq_nat count 0))).
 Proof.
   intros * is_dec ** .
 
@@ -1302,8 +768,8 @@ Proof.
   setoid_rewrite refine_decide_negation.
   setoid_rewrite tupleAgree_equivalence.
   setoid_rewrite (@refine_constraint_check_into_query _ _
-                    (fun (x: Tuple ) => tupleAgree_computational x ref args1 /\
-                                        ~ tupleAgree_computational x ref args2)); try assumption.
+                                                      (fun (x: Tuple ) => tupleAgree_computational x ref args1 /\
+                                                                          ~ tupleAgree_computational x ref args2)); try assumption.
 
   Opaque Query_For Count.
   simplify with monad laws.
@@ -1313,18 +779,18 @@ Qed.
 
 
 Theorem FunctionalDependency_symmetry
-: forall A H (f : _ -> _ -> Comp A) (P : _ -> Prop) attrlist1 attrlist2 n,
+  : forall A H (f : _ -> _ -> Comp A) (P : _ -> Prop) attrlist1 attrlist2 n,
     refine (x1 <- {b | decides b
                                (forall tup' : @IndexedTuple H,
-                                  P tup'
-                                  -> FunctionalDependency_P attrlist1 attrlist2 n (indexedElement tup'))};
+                                   P tup'
+                                   -> FunctionalDependency_P attrlist1 attrlist2 n (indexedElement tup'))};
             x2 <- {b | decides b (forall tup' : @IndexedTuple H,
-                                    P tup'
-                                    -> FunctionalDependency_P attrlist1 attrlist2 (indexedElement tup') n)};
+                                     P tup'
+                                     -> FunctionalDependency_P attrlist1 attrlist2 (indexedElement tup') n)};
             f x1 x2)
            (x1 <- {b | decides b (forall tup' : @IndexedTuple H,
-                                    P tup'
-                                    -> FunctionalDependency_P attrlist1 attrlist2 n (indexedElement tup'))};
+                                     P tup'
+                                     -> FunctionalDependency_P attrlist1 attrlist2 n (indexedElement tup'))};
             f x1 x1).
 Proof.
   unfold refine, FunctionalDependency_P; intros.
@@ -1338,7 +804,7 @@ Proof.
 Qed.
 
 Lemma if_duplicate_cond_eq {A}
-: forall (i : bool) (t e : A),
+  : forall (i : bool) (t e : A),
     (if i then (if i then t else e) else e) = if i then t else e.
 Proof.
   destruct i; reflexivity.
@@ -1349,10 +815,10 @@ Global Instance nil_List_Query_eq :
   {| As_Query_eq := inil _ |}.
 
 Global Instance cons_List_Query_eq
-         {A : Type}
-         {As : list Type}
-         {A_Query_eq : Query_eq A}
-         {As_Query_eq' : List_Query_eq As}
-:
-  List_Query_eq (A :: As) :=
+       {A : Type}
+       {As : list Type}
+       {A_Query_eq : Query_eq A}
+       {As_Query_eq' : List_Query_eq As}
+  :
+    List_Query_eq (A :: As) :=
   {| As_Query_eq := icons _ A_Query_eq As_Query_eq |}.
