src/QueryStructure/Implementation/Operations/General/InsertRefinements.v
@@ -1,6 +1,7 @@
 Require Import Coq.Strings.String Coq.omega.Omega Coq.Lists.List
         Coq.Logic.FunctionalExtensionality Coq.Sets.Ensembles
         Fiat.Computation
+        Fiat.Computation.Refinements.Iterate_Decide_Comp
         Fiat.ADT
         Fiat.ADTRefinement
         Fiat.ADTNotation
